Fix i2cRegsCircuitProofTheory with window support
I did end up allowing i2c_tick to return errors in the case of
situations we don't model, and also changing it to do so (mostly to make
sure the shape of i2c_cheshire_run_ISR_fnums was realistic).

I also removed cheshire_run_cheshire_req_ISR: the statement I changed it
to after adding window support was useless, since there will be many
states (e.g. when enabletarget is 1 with i2c) which i2c_tick will always
reject regardless of the value of `notif`.

util/gen_mappings.py
@@ -1,3 +1,6 @@
+# TODO: maybe remove the unused nb argument from read and the unused st argument
+# from write?
+
 import sys
 from math import ceil
 
