i2c/i2cRegsCircuitProofScript.sml
@@ -1,11 +1,205 @@
 open HolKernel Parse boolLib bossLib;
 open BasicProvers wordsLib;
 open wordsTheory;
-open translatorTheory;
+open sumExtraTheory translatorTheory;
 open cheshireCircuitTheory cheshireOracleTheory i2cCircuitTheory i2cCircuitStateTheory i2cCoreTheory i2cMappingsTheory i2cRegsTheory i2cRegsCommTheory;
 
 val _ = new_theory "i2cRegsCircuitProof";
 
+(* Peripheral-independent section *)
+Theorem i2c_read_fnums:
+  i2c_read (st with fnums := fnums) nb offset = i2c_read st nb offset
+Proof
+  asm_simp_tac std_ss [i2c_read_def]
+  >> asm_simp_tac std_ss [i2c_get_status_fmtfull_def, i2c_get_status_rxfull_def, i2c_get_status_fmtempty_def, i2c_get_status_hostidle_def, i2c_get_status_targetidle_def, i2c_get_status_rxempty_def, i2c_get_status_txfull_def, i2c_get_status_acqfull_def, i2c_get_status_txempty_def, i2c_get_status_acqempty_def, i2c_get_rdata_rdata_def, i2c_get_fifo_status_fmtlvl_def, i2c_get_fifo_status_txlvl_def, i2c_get_fifo_status_rxlvl_def, i2c_get_fifo_status_acqlvl_def, i2c_get_val_scl_rx_def, i2c_get_val_sda_rx_def, i2c_get_acqdata_abyte_def, i2c_get_acqdata_signal_def]
+  >> asm_simp_tac std_ss [i2c_state_accfupds]
+QED
+
+Theorem i2c_write_fnums:
+  i2c_write (st with fnums := fnums) nb offset wdata = i2c_write st nb offset wdata
+Proof
+  asm_simp_tac std_ss [i2c_write_def, i2c_state_accfupds]
+QED
+
+Theorem i2c_cheshire_req_fnums:
+  cheshire_req i2c_read i2c_write (st with fnums := fnums) req =
+  cheshire_req i2c_read i2c_write st req
+Proof
+  simp [cheshire_req_def, i2c_read_fnums, i2c_write_fnums]
+QED
+
+Theorem i2c_read_ISR:
+  ISR (i2c_read st nb offset) = ISR (i2c_read st' nb offset)
+Proof
+  asm_simp_tac std_ss [i2c_read_def]
+  >> rpt (IF_CASES_TAC >- asm_simp_tac std_ss [])
+  >> asm_simp_tac std_ss []
+QED
+
+Theorem i2c_write_ISR:
+  ISR (i2c_write st nb offset wdata) = ISR (i2c_write st' nb offset wdata)
+Proof
+  asm_simp_tac std_ss [i2c_write_def]
+  >> rpt (IF_CASES_TAC >- asm_simp_tac std_ss [])
+  >> asm_simp_tac std_ss []
+QED
+
+Theorem i2c_cheshire_req_ISR:
+  ISR (cheshire_req i2c_read i2c_write st req) =
+  ISR (cheshire_req i2c_read i2c_write st' req)
+Proof
+  simp [cheshire_req_def]
+  >> ntac 4 CASE_TAC
+  >- simp [ISR_SUM_MAP, i2c_read_ISR]
+  >- simp [ISR_SUM_MAP, i2c_write_ISR]
+QED
+
+Theorem INR_imp_ISR:
+  x = INR y ==> ISR x
+Proof
+  simp []
+QED
+
+Theorem i2c_read_unchanged:
+  i2c_read st nb offset = INR (notif, rdata) ==>
+  ?rdata'. i2c_read st' nb' offset = INR (notif, rdata')
+Proof
+  asm_simp_tac std_ss [i2c_read_def]
+  >> rpt (IF_CASES_TAC >- asm_simp_tac std_ss [])
+  >> asm_simp_tac std_ss []
+QED
+
+Theorem i2c_write_unchanged:
+  i2c_write st nb offset wdata = INR (st_upd, notif) ==>
+  i2c_write st' nb offset wdata = INR (st_upd, notif)
+Proof
+  asm_simp_tac std_ss [i2c_write_def]
+QED
+
+Theorem i2c_cheshire_req_unchanged:
+  cheshire_req i2c_read i2c_write st req = INR (st_upd, notif, rdata) ==>
+  ?rdata'.
+  cheshire_req i2c_read i2c_write st' req = INR (st_upd, notif, rdata')
+Proof
+  rpt strip_tac
+  >> fs [cheshire_req_def]
+  >> rpt CASE_TAC
+  (* noop *)
+  >- fs []
+  (* read *)
+  >- (fs []
+      >> (Cases_on `i2c_read st q q'` >- fs [])
+      >> fs []
+      >> pairarg_tac
+      >> gvs []
+      >> drule_then (qspecl_then [`st'`, `q`] strip_assume_tac) i2c_read_unchanged
+      >> simp [])
+  (* write *)
+  >- (fs []
+      >> (Cases_on `i2c_write st q q' x` >- fs [])
+      >> fs []
+      >> pairarg_tac
+      >> gvs []
+      >> drule_then (qspec_then `st'` assume_tac) i2c_write_unchanged
+      >> simp [])
+QED
+
+Theorem SUM_MAP_INR:
+  SUM_MAP f g x = INR y <=> ?z. x = INR z /\ g z = y
+Proof
+  Cases_on `x` >> simp []
+QED
+
+(* Peripheral-specific section (things that I would put in *CoreTheory if I
+ * could, but which depend on things defined later) *)
+Theorem i2c_tick_ISR_ctrl_enabletarget:
+  st.regs.ctrl.enabletarget = st'.regs.ctrl.enabletarget ==>
+  ISR (i2c_tick notif st) = ISR (i2c_tick notif st')
+Proof
+  Cases_on `st'.regs.ctrl.enabletarget = 1w` >> simp [i2c_tick_def]
+QED
+
+Theorem i2c_write_ctrl_enabletarget:
+  i2c_write st nb offset wdata = INR (st_upd, notif) /\
+  i2c_write st' nb offset wdata = INR (st_upd', notif') /\
+  st''.regs.ctrl.enabletarget = st'''.regs.ctrl.enabletarget ==>
+  (st_upd st'').regs.ctrl.enabletarget = (st_upd' st''').regs.ctrl.enabletarget
+Proof
+  rpt strip_tac
+  >> rpt (dxrule_then assume_tac i2c_write_st_upd_alt)
+  >> simp []
+QED
+
+Theorem i2c_cheshire_req_ctrl_enabletarget:
+  cheshire_req i2c_read i2c_write st req = INR (st_upd, notif, rdata) /\
+  cheshire_req i2c_read i2c_write st' req = INR (st_upd', notif', rdata') /\
+  st''.regs.ctrl.enabletarget = st'''.regs.ctrl.enabletarget ==>
+  (st_upd st'').regs.ctrl.enabletarget = (st_upd' st''').regs.ctrl.enabletarget
+Proof
+  simp [cheshire_req_def]
+  >> rpt CASE_TAC
+  >- simp []
+  >- (rpt strip_tac
+      >> fs [SUM_MAP_INR]
+      >> rpt (pairarg_tac >> gvs []))
+  >- (rpt strip_tac
+      >> fs [SUM_MAP_INR]
+      >> rpt (pairarg_tac >> gvs [])
+      >> irule i2c_write_ctrl_enabletarget
+      >> simp []
+      >> rpt (goal_assum $ drule_at Any))
+QED
+
+Theorem i2c_cheshire_run_ISR_fnums:
+  ISR (cheshire_run i2c_tick i2c_read i2c_write (st with fnums := fnums) reqs) =
+  ISR (cheshire_run i2c_tick i2c_read i2c_write st reqs)
+Proof
+  goal_term (fn tm =>
+    `^tm /\ (ISR (cheshire_run i2c_tick i2c_read i2c_write st reqs) ==>
+    (FST (OUTR (cheshire_run i2c_tick i2c_read i2c_write (st with fnums := fnums) reqs))).regs.ctrl.enabletarget
+    = (FST (OUTR (cheshire_run i2c_tick i2c_read i2c_write st reqs))).regs.ctrl.enabletarget)`
+    suffices_by simp [])
+  >> qid_spec_tac `st`
+  >> qid_spec_tac `fnums`
+  >> Induct_on `reqs` using listTheory.SNOC_INDUCT
+  >- simp [cheshire_run_def]
+  >- (rpt gen_tac
+      >> conj_asm1_tac
+      >- (iff_tac
+          >> rpt strip_tac
+          >> fs [cheshire_run_ISR_SNOC]
+
+          (* Apply the inductive hypothesis to prove that the other cheshire_run is also INR *)
+          >> qpat_assum `cheshire_run _ _ _ _ _ = INR _` (fn thm => assume_tac (MATCH_MP INR_imp_ISR thm))
+          >| [
+            last_assum (fn thm => drule_then assume_tac (iffLR (cj 1 thm))),
+            last_assum (fn thm => drule_then (qspec_then `fnums` assume_tac) (iffRL (cj 1 thm)))
+          ]
+          >> dxrule_then strip_assume_tac (iffLR ISR_exists)
+          >> PairCases_on `x'`
+          >> simp []
+
+          (* Obtain the other st_upd, notif and rdata *)
+          >> drule_then (qspec_then `x'0` strip_assume_tac) i2c_cheshire_req_unchanged
+          >> simp []
+
+          (* Apply the inductive hypothesis to prove that the other i2c_tick is also INR *)
+          >> last_x_assum $ qspecl_then [`fnums`, `st`] strip_assume_tac
+          >> rfs []
+          >> drule_then assume_tac i2c_tick_ISR_ctrl_enabletarget
+          >> fs [])
+      >- (first_x_assum (assume_tac o iffRL)
+          >> rpt strip_tac
+          >> last_x_assum (fn thm => fs [ISR_exists] >> qspecl_then [`fnums`, `st`] strip_assume_tac thm)
+          >> rfs [cheshire_run_SNOC, sum_bind_INR]
+          >> rpt (pairarg_tac >> gvs [sum_bind_INR])
+          >> irule i2c_cheshire_req_ctrl_enabletarget
+          >> ntac 2 $ dxrule_then (fn thm => simp [thm]) i2c_tick_hwro_unchanged
+          >> qexistsl [`notif'`, `notif`, `rdata'`, `rdata`, `x`, `st'³'`, `st'`]
+          >> simp []))
+QED
+
+(* Peripheral-independent section *)
 Theorem procs_append:
   procs (ps ++ qs) fext s s' = procs qs fext s (procs ps fext s s')
 Proof
@@ -199,7 +393,7 @@ Theorem i2c_reg_top_rsp_ready_error_inner:
       s''.reg2hw = s'.reg2hw /\ s''.regs = s'.regs /\ s''.reg_rsp_o = s'.reg_rsp_o
       /\ s''.addr = s'.addr /\ s''.write = s'.write /\ s''.wdata = s'.wdata
       /\ s''.wstrb = s'.wstrb /\ s''.valid = s'.valid /\ s''.error = s'.error)
-  ==> rsp.ready /\ rsp.error = i2c_req_error req
+  ==> rsp.ready /\ (rsp.error ==> i2c_req_error req \/ i2c_win_error (i2c fext fbits n).win_buses)
 Proof
   qpat_abbrev_tac `sstep = procs (_ ++ ffs2)`
   >> qpat_abbrev_tac `cstep = procs (_ ++ [i2c_reg_top_comb_2])`
@@ -211,54 +405,6 @@ Proof
 QED
 
 Theorem i2c_reg_top_rsp_ready_error = SRULE [SF boolSimps.LET_ss] i2c_reg_top_rsp_ready_error_inner;
-
-Theorem i2c_reg_top_rsp_correct_inner:
-  let
-    i2c = mk_module (procs (ffs1 ++ [i2c_reg_top_ff] ++ ffs2)) (procs ([i2c_reg_top_comb_1] ++ combs ++ [i2c_reg_top_comb_2])) i2c_circuit_init;
-    req_c = reg_req_decode (fext n).reg_req_i: 7 reg_req;
-    oracle_res = cheshire_req i2c_read i2c_write st req_m;
-    rsp = reg_rsp_decode (i2c fext fbits n).reg_rsp_o;
-  in
-  (!proc fext s s'. MEM proc (ffs1 ++ ffs2 ++ combs) ==>
-    let
-      s'' = proc fext s s'
-    in
-      s''.reg2hw = s'.reg2hw /\ s''.regs = s'.regs /\ s''.reg_rsp_o = s'.reg_rsp_o
-      /\ s''.addr = s'.addr /\ s''.write = s'.write /\ s''.wdata = s'.wdata
-      /\ s''.wstrb = s'.wstrb /\ s''.valid = s'.valid /\ s''.error = s'.error)
-  /\ i2c_state_rel st (i2c fext fbits n)
-  /\ cheshire_req_rel req_m req_c
-  ==> rsp.ready
-    /\ rsp.error = ISL oracle_res
-    /\ (!st_upd notif rdata. oracle_res = INR (st_upd, notif, SOME rdata) ==> rsp.rdata = rdata)
-Proof
-  simp []
-  >> qpat_abbrev_tac `sstep = procs (_ ++ ffs2)`
-  >> qpat_abbrev_tac `cstep = procs (i2c_reg_top_comb_1::_)`
-  >> rpt strip_tac
-  >> `?s'. mk_circuit sstep cstep (i2c_circuit_init fbits) fext n = cstep (fext n) s' s'` by irule mk_circuit_cstep
-  >> unabbrev_all_tac
-  >> drule_then assume_tac i2c_reg_top_rsp_ready_error
-  >> simp []
-  (* error *)
-  >- simp [cheshire_req_i2c_req_error]
-  (* rdata *)
-  >- (fs [mk_module_def, procs_def, procs_append, reg_rsp_decode_def]
-      >> drule_then strip_assume_tac cheshire_req_INR_cases
-      >- fs []
-      >- (dep_rewrite.DEP_REWRITE_TAC [i2c_reg_top_comb_2_i2c_read]
-          >> `!fext s s'. (i2c_reg_top_comb_1 fext s s').regs = s'.regs` by simp [i2c_reg_top_comb_1_flat]
-          >> `!fext s s'. (i2c_reg_top_comb_2 fext s s').regs = s'.regs` by simp [i2c_reg_top_comb_2_flat]
-          >> `st.regs = (i2c_reg_top_comb_2 (fext n) s' (procs combs (fext n) s' (i2c_reg_top_comb_1 (fext n) s' s'))).regs` by fs [i2c_state_rel_def, i2c_core_state_rel_def]
-          >> rfs [procs_unchanged]
-          >> `!fext s s'. (i2c_reg_top_comb_2 fext s s').hw2reg = s'.hw2reg` by simp [i2c_reg_top_comb_2_flat]
-          >> `i2c_hwext_read_rel st (i2c_reg_top_comb_2 (fext n) s' (procs combs (fext n) s' (i2c_reg_top_comb_1 (fext n) s' s'))).hw2reg` by fs [i2c_state_rel_def, i2c_core_state_rel_def]
-          >> gs [cheshire_req_rel_read]
-          >> simp [i2c_reg_top_comb_1_flat, cheshire_req_def])
-      >- fs [])
-QED
-
-Theorem i2c_reg_top_rsp_correct = SRULE [SF boolSimps.LET_ss] i2c_reg_top_rsp_correct_inner;
 
 Theorem i2c_write_i2c_hwext_notif_rel:
   cheshire_req_rel (SOME (nb, offset, SOME wdata)) req /\
@@ -286,6 +432,95 @@ Proof
   >> rpt TOP_CASE_TAC
   >> fs [i2c_hwext_notif_rel_def, i2c_req_error_def, w2n_eq_iff_eq_n2w]
 QED
+
+Theorem cheshire_req_i2c_hwext_notif_rel:
+  cheshire_req_rel req_m req_c /\
+  cheshire_req i2c_read i2c_write st req_m = INR (_, notif, _) ==>
+  i2c_hwext_notif_rel notif req_c
+Proof
+  rpt strip_tac
+  >> drule_then strip_assume_tac cheshire_req_INR_cases
+  >- fs [cheshire_req_rel_def, i2c_hwext_notif_rel_def, i2c_req_error_def]
+  >- (fs [] >> drule_all i2c_read_i2c_hwext_notif_rel >> simp [])
+  >- (fs [] >> drule_all i2c_write_i2c_hwext_notif_rel >> simp [])
+QED
+
+Theorem i2c_reg_top_rsp_correct_inner:
+  let
+    i2c = mk_module (procs (ffs1 ++ [i2c_reg_top_ff] ++ ffs2)) (procs ([i2c_reg_top_comb_1] ++ combs ++ [i2c_reg_top_comb_2])) i2c_circuit_init;
+    req_c = reg_req_decode (fext n).reg_req_i: 7 reg_req;
+    oracle_res = cheshire_req i2c_read i2c_write st req_m;
+    rsp = reg_rsp_decode (i2c fext fbits n).reg_rsp_o;
+  in
+  (!proc fext s s'. MEM proc (ffs1 ++ ffs2 ++ combs) ==>
+    let
+      s'' = proc fext s s'
+    in
+      s''.reg2hw = s'.reg2hw /\ s''.regs = s'.regs /\ s''.reg_rsp_o = s'.reg_rsp_o
+      /\ s''.addr = s'.addr /\ s''.write = s'.write /\ s''.wdata = s'.wdata
+      /\ s''.wstrb = s'.wstrb /\ s''.valid = s'.valid /\ s''.error = s'.error)
+  /\ (!st req_m fext fbits n st_upd notif rdata.
+    let
+      req_c = reg_req_decode (fext n).reg_req_i: 7 reg_req
+    in
+    i2c_state_rel st (i2c fext fbits n)
+    /\ cheshire_req_rel req_m req_c
+    /\ cheshire_req i2c_read i2c_write st req_m = INR (st_upd, notif, rdata)
+    /\ ISR (i2c_tick notif st)
+    (* TODO: the other way to do this would be to compare notif to
+     * (i2c_reg_top_comb_1 (fext n) (i2c fext fbits n) (i2c fext fbits n)).reg2hw;
+     * that has the advantage of being closer to what i2c_core actually operates
+     * on, but is also uglier.
+     *
+     * So, we can try switching to that if this way turns out to be annoying. *)
+    /\ i2c_hwext_notif_rel notif req_c
+    (* Note: somewhat counterintuitively, this actually shows that
+     * i2c_hwext_read_rel is true for the next clock cycle, not this one. *)
+    ==> ?fnums. i2c_core_state_rel (st_upd (OUTR (i2c_tick notif (st with fnums := fnums)))) (i2c fext fbits (SUC n))
+      (* Note: this is only true because st_upd hasn't run yet, otherwise software
+       * might have overwritten some stuff and made this false. *)
+      /\ i2c_hw_write_rel (st with fnums := fnums).regs (OUTR (i2c_tick notif (st with fnums := fnums))).regs
+                          (i2c fext fbits n).hw2reg
+      /\ ~i2c_win_error (i2c fext fbits n).win_buses)
+  /\ i2c_state_rel st (i2c fext fbits n)
+  /\ cheshire_req_rel req_m req_c
+  ==> rsp.ready
+    /\ (!st_upd notif rdata. oracle_res = INR (st_upd, notif, rdata) ==>
+      (rsp.error ==> ISL (i2c_tick notif st)) /\
+      (!value. rdata = SOME value ==> rsp.rdata = value))
+Proof
+  simp []
+  >> qpat_abbrev_tac `sstep = procs (_ ++ ffs2)`
+  >> qpat_abbrev_tac `cstep = procs (i2c_reg_top_comb_1::_)`
+  >> rpt strip_tac
+  >> `?s'. mk_circuit sstep cstep (i2c_circuit_init fbits) fext n = cstep (fext n) s' s'` by irule mk_circuit_cstep
+  >> unabbrev_all_tac
+  >> drule_then assume_tac i2c_reg_top_rsp_ready_error
+  >> simp []
+  (* error *)
+  >- (first_x_assum (drule_then strip_assume_tac o cj 2)
+      >- (`~ISL (cheshire_req i2c_read i2c_write st req_m)` by simp []
+          >> drule_then (fn thm => full_simp_tac pure_ss [thm]) cheshire_req_i2c_req_error)
+      >- (drule_all_then assume_tac cheshire_req_i2c_hwext_notif_rel
+          >> spose_not_then (assume_tac o SRULE [])
+          >> qpat_x_assum `∀st req_m fext fbits n st_upd notif rdata. _` $ drule_all_then strip_assume_tac))
+  (* rdata *)
+  >- (fs [mk_module_def, procs_def, procs_append, reg_rsp_decode_def]
+      >> drule_then strip_assume_tac cheshire_req_INR_cases
+      >- fs []
+      >- (dep_rewrite.DEP_REWRITE_TAC [i2c_reg_top_comb_2_i2c_read]
+          >> `!fext s s'. (i2c_reg_top_comb_1 fext s s').regs = s'.regs` by simp [i2c_reg_top_comb_1_flat]
+          >> `!fext s s'. (i2c_reg_top_comb_2 fext s s').regs = s'.regs` by simp [i2c_reg_top_comb_2_flat]
+          >> `st.regs = (i2c_reg_top_comb_2 (fext n) s' (procs combs (fext n) s' (i2c_reg_top_comb_1 (fext n) s' s'))).regs` by fs [i2c_state_rel_def, i2c_core_state_rel_def]
+          >> rfs [procs_unchanged]
+          >> `!fext s s'. (i2c_reg_top_comb_2 fext s s').hw2reg = s'.hw2reg` by simp [i2c_reg_top_comb_2_flat]
+          >> `i2c_hwext_read_rel st (i2c_reg_top_comb_2 (fext n) s' (procs combs (fext n) s' (i2c_reg_top_comb_1 (fext n) s' s'))).hw2reg` by fs [i2c_state_rel_def, i2c_core_state_rel_def]
+          >> gs [cheshire_req_rel_read]
+          >> simp [i2c_reg_top_comb_1_flat, cheshire_req_def])
+      >- fs [])
+QED
+
+Theorem i2c_reg_top_rsp_correct = SRULE [SF boolSimps.LET_ss] i2c_reg_top_rsp_correct_inner;
 
 Theorem i2c_parsed_signals_inner:
   let
@@ -343,46 +578,40 @@ Theorem i2c_reg_top_i2c_state_rel_step_inner:
     i2c_state_rel st (i2c fext fbits n)
     /\ cheshire_req_rel req_m req_c
     /\ cheshire_req i2c_read i2c_write st req_m = INR (st_upd, notif, rdata)
-    (* TODO: the other way to do this would be to compare notif to
-     * (i2c_reg_top_comb_1 (fext n) (i2c fext fbits n) (i2c fext fbits n)).reg2hw;
-     * that has the advantage of being closer to what i2c_core actually operates
-     * on, but is also uglier.
-     *
-     * So, we can try switching to that if this way turns out to be annoying. *)
+    /\ ISR (i2c_tick notif st)
     /\ i2c_hwext_notif_rel notif req_c
-    (* Note: somewhat counterintuitively, this actually shows that
-     * i2c_hwext_read_rel is true for the next clock cycle, not this one. *)
-    ==> ?fnums. i2c_core_state_rel (st_upd (i2c_tick notif (st with fnums := fnums))) (i2c fext fbits (SUC n))
-      (* Note: this is only true because st_upd hasn't run yet, otherwise software
-       * might have overwritten some stuff and made this false. *)
-      /\ i2c_hw_write_rel (st with fnums := fnums).regs (i2c_tick notif (st with fnums := fnums)).regs
-                          (i2c fext fbits n).hw2reg)
+    ==> ?fnums. i2c_core_state_rel (st_upd (OUTR (i2c_tick notif (st with fnums := fnums)))) (i2c fext fbits (SUC n))
+      /\ i2c_hw_write_rel (st with fnums := fnums).regs (OUTR (i2c_tick notif (st with fnums := fnums))).regs
+                          (i2c fext fbits n).hw2reg
+      /\ ~i2c_win_error (i2c fext fbits n).win_buses)
   /\ i2c_state_rel st (i2c fext fbits n)
   /\ cheshire_req_rel req_m req_c
   /\ cheshire_req i2c_read i2c_write st req_m = INR (st_upd, notif, rdata)
-  ==> ?fnums. i2c_state_rel (st_upd (i2c_tick notif (st with fnums := fnums))) (i2c fext fbits (SUC n))
+  /\ ISR (i2c_tick notif st)
+  ==> ?fnums. i2c_state_rel (st_upd (OUTR (i2c_tick notif (st with fnums := fnums)))) (i2c fext fbits (SUC n))
 Proof
   simp []
   >> rpt strip_tac
 
   >> drule_all_then strip_assume_tac i2c_reg_top_rsp_correct
-  >> drule_then assume_tac i2c_parsed_signals
-  >> drule_then assume_tac i2c_reg_top_rsp_ready_error
-
-  >> qabbrev_tac `req_c = reg_req_decode (fext n).reg_req_i: 7 reg_req`
-
-  >> `i2c_hwext_notif_rel notif req_c`
-     by (drule_then strip_assume_tac cheshire_req_INR_cases
-         >- fs [cheshire_req_rel_def, i2c_hwext_notif_rel_def, i2c_req_error_def]
-         >- (fs [] >> drule_all i2c_read_i2c_hwext_notif_rel >> simp [])
-         >- (fs [] >> drule_all i2c_write_i2c_hwext_notif_rel >> simp []))
+  >> drule_then (qspecl_then [`n`, `fext`, `fbits`] strip_assume_tac) i2c_parsed_signals
+  >> drule_then (qspecl_then [`n`, `fext`, `fbits`] strip_assume_tac) i2c_reg_top_rsp_ready_error
+  >> drule_all_then assume_tac cheshire_req_i2c_hwext_notif_rel
 
   (* We need to do this in all cases so we can pick the value of fnums. *)
-  >> fs [Abbr `req_c`]
-  >> qpat_x_assum `!st nb fext fbits n st_upd notif rdata. _ ==> ?fnums. _`
+  >> qpat_x_assum `!st req_m fext fbits n st_upd notif rdata. _ ==> ?fnums. _`
        $ drule_all_then strip_assume_tac
   >> qabbrev_tac `req_c = reg_req_decode (fext n).reg_req_i: 7 reg_req`
   >> qexists `fnums`
+
+  >> `?st'. i2c_tick notif (st with fnums := fnums) = INR st'`
+     by (irule (iffLR ISR_exists) >> simp [i2c_tick_ISR_fnums])
+  >> qmatch_asmsub_abbrev_tac `rsp.ready`
+  >> `~rsp.error`
+     by (spose_not_then assume_tac
+         >> `~ISL (cheshire_req i2c_read i2c_write st req_m)` by simp []
+         >> drule_then (fn thm => full_simp_tac bool_ss [thm]) cheshire_req_i2c_req_error)
+  >> fs [Abbr `rsp`]
 
   >> simp [i2c_state_rel_def]
   >> rpt strip_tac
@@ -400,13 +629,17 @@ Proof
           >> simp [i2c_reg_top_ff_flat, procs_unchanged]
           (* TODO: auto-generate this (probably need to make a new *Lib.sml to put it in...) *)
           >> simp [i2c_regs_component_equality, i2c_intr_state_component_equality, i2c_intr_enable_component_equality, i2c_ctrl_component_equality, i2c_fdata_component_equality, i2c_fifo_ctrl_component_equality, i2c_ovrd_component_equality, i2c_timing0_component_equality, i2c_timing1_component_equality, i2c_timing2_component_equality, i2c_timing3_component_equality, i2c_timing4_component_equality, i2c_timeout_ctrl_component_equality, i2c_target_id_component_equality, i2c_txdata_component_equality, i2c_host_timeout_ctrl_component_equality]
-          >> gs [i2c_state_rel_def, i2c_tick_hwro_unchanged, i2c_hw_write_rel_def])
+          >> gs [i2c_state_rel_def, i2c_hw_write_rel_def]
+          >> drule_then strip_assume_tac i2c_tick_hwro_unchanged
+          >> simp [])
       >- (fs [cheshire_req_rel_write]
           >> drule i2c_write_st_upd_alt
-          (* TODO: I think the reason this doesn't work for SPI might be that 
+          (* TODO: I think the reason this doesn't work for SPI might be that
            * procs_unchanged isn't applying properly or something? *)
           >> simp [i2c_reg_top_ff_flat, procs_unchanged]
-          >> fs [i2c_state_rel_def, i2c_tick_hwro_unchanged, i2c_hw_write_rel_def, reg_rsp_decode_def, w2n_eq_iff_eq_n2w]))
+          >> fs [i2c_state_rel_def, i2c_hw_write_rel_def, reg_rsp_decode_def, w2n_eq_iff_eq_n2w]
+          >> drule_then strip_assume_tac i2c_tick_hwro_unchanged
+          >> simp []))
   (* buffered_notif *)
   >- (simp [mk_module_def, mk_circuit_def, procs_def, procs_append, i2c_reg_top_comb_2_flat]
       >> simp [procs_unchanged, i2c_reg_top_comb_1_flat]
@@ -417,36 +650,17 @@ Proof
       >> drule_then strip_assume_tac cheshire_req_INR_st_upd_cases
 
       >- (drule_then (fn thm => full_simp_tac pure_ss [thm]) cheshire_req_rel_valid_write
-          >> simp [i2c_tick_buffered_notif_NONE])
+          >> drule_then assume_tac i2c_tick_buffered_notif_NONE
+          >> simp [])
       >- (fs [cheshire_req_rel_write]
           >> drule i2c_write_st_upd_alt
           >> simp []
           >> rpt (IF_CASES_TAC >- fs [w2n_eq_iff_eq_n2w])
-          >> fs [i2c_tick_buffered_notif_NONE, w2n_eq_iff_eq_n2w]))
+          >> drule_then assume_tac i2c_tick_buffered_notif_NONE
+          >> fs [w2n_eq_iff_eq_n2w]))
 QED
 
 Theorem i2c_reg_top_i2c_state_rel_step = SRULE [SF boolSimps.LET_ss] i2c_reg_top_i2c_state_rel_step_inner;
-
-Theorem i2c_read_fnums:
-  i2c_read (st with fnums := fnums) nb offset = i2c_read st nb offset
-Proof
-  asm_simp_tac std_ss [i2c_read_def]
-  >> asm_simp_tac std_ss [i2c_get_status_fmtfull_def, i2c_get_status_rxfull_def, i2c_get_status_fmtempty_def, i2c_get_status_hostidle_def, i2c_get_status_targetidle_def, i2c_get_status_rxempty_def, i2c_get_status_txfull_def, i2c_get_status_acqfull_def, i2c_get_status_txempty_def, i2c_get_status_acqempty_def, i2c_get_rdata_rdata_def, i2c_get_fifo_status_fmtlvl_def, i2c_get_fifo_status_txlvl_def, i2c_get_fifo_status_rxlvl_def, i2c_get_fifo_status_acqlvl_def, i2c_get_val_scl_rx_def, i2c_get_val_sda_rx_def, i2c_get_acqdata_abyte_def, i2c_get_acqdata_signal_def]
-  >> asm_simp_tac std_ss [i2c_state_accfupds]
-QED
-
-Theorem i2c_write_fnums:
-  i2c_write (st with fnums := fnums) nb offset wdata = i2c_write st nb offset wdata
-Proof
-  asm_simp_tac std_ss [i2c_write_def, i2c_state_accfupds]
-QED
-
-Theorem i2c_cheshire_req_fnums:
-  cheshire_req i2c_read i2c_write (st with fnums := fnums) req =
-  cheshire_req i2c_read i2c_write st req
-Proof
-  simp [cheshire_req_def, i2c_read_fnums, i2c_write_fnums]
-QED
 
 Theorem OUTR_SUM_MAP:
   ISR z ==> OUTR (SUM_MAP f g z) = g (OUTR z)
@@ -476,34 +690,37 @@ Proof
   >> last_x_assum (fn thm => simp [Once thm])
 QED
 
-Theorem cheshire_run_unused_fnums_2:
-  (!st req. MEM req reqs ==> ISR (cheshire_req i2c_read i2c_write st req)) ==>
-  ?n st' rdatas. !fnums. (!i. i < n ==> fnums i = st.fnums i) ==>
+Theorem cheshire_run_unused_fnums:
+  cheshire_run i2c_tick i2c_read i2c_write st reqs = INR (st', rdatas) ==>
+  ?n. !fnums. (!i. i < n ==> fnums i = st.fnums i) ==>
   cheshire_run i2c_tick i2c_read i2c_write (st with fnums := fnums) reqs = INR (st' with fnums := (\i. fnums (i + n)), rdatas)
 Proof
   qid_spec_tac `st`
+  >> qid_spec_tac `st'`
+  >> qid_spec_tac `rdatas`
   >> Induct_on `reqs`
   >- (rpt strip_tac
-      >> qexistsl [`0`, `st`, `[]`]
-      >> simp [cheshire_run_def, SF ETA_ss])
-  >- (simp [cheshire_run_def]
-      >> rpt strip_tac
-      >> `?oracle_res. cheshire_req i2c_read i2c_write st h = INR oracle_res` by simp [GSYM sumExtraTheory.ISR_exists]
-      >> PairCases_on `oracle_res`
-      >> fs [i2c_cheshire_req_fnums]
+      >> qexists `0`
+      >> fs [cheshire_run_def, SF ETA_ss])
+  >- (rpt strip_tac
+      >> fs [cheshire_run_INR_CONS, i2c_cheshire_req_fnums]
 
-      >> strip_assume_tac $ Q.INST [`notif` |-> `oracle_res1`] i2c_tick_unused_fnums
+      >> strip_assume_tac i2c_tick_unused_fnums
       >> qrefine `n + m`
-      >> simp []
+      >> rfs []
+
       >> drule_then assume_tac i2c_st_upd_fnums_fupd
       >> simp []
-      >> last_x_assum $ qspec_then `oracle_res0 (i2c_tick oracle_res1 st)` strip_assume_tac
+      >> last_x_assum $ drule_then strip_assume_tac
       >> qexists `n'`
-      >> drule_then assume_tac unused_fnums_ignored_fnums_val
       >> drule_then assume_tac i2c_st_upd_fnums
       >> fs []
-      >> qexistsl [`st'`, `oracle_res2::rdatas`]
-      >> simp [])
+      >> `st''.fnums = (\i. st.fnums (i + n))`
+         by (qpat_x_assum `!fnums. _ ==> i2c_tick _ _ = _` $ qspec_then `st.fnums` assume_tac
+             >> `st with fnums := st.fnums = st` by simp [i2c_state_component_equality]
+             >> fs []
+             >> qpat_x_assum `_ = st''` (fn thm => simp [Once (GSYM thm)]))
+      >> fs [])
 QED
 
 (* If the initial model state lines up with `i2c_circuit_init`, and all the
@@ -528,19 +745,19 @@ Theorem i2c_reg_top_correct:
     i2c_state_rel st (i2c fext fbits n)
     /\ cheshire_req_rel req_m req_c
     /\ cheshire_req i2c_read i2c_write st req_m = INR (st_upd, notif, rdata)
+    /\ ISR (i2c_tick notif st)
     /\ i2c_hwext_notif_rel notif req_c
-    ==> ?fnums. i2c_core_state_rel (st_upd (i2c_tick notif (st with fnums := fnums))) (i2c fext fbits (SUC n))
-      /\ i2c_hw_write_rel (st with fnums := fnums).regs (i2c_tick notif (st with fnums := fnums)).regs
-                          (i2c fext fbits n).hw2reg)
+    ==> ?fnums. i2c_core_state_rel (st_upd (OUTR (i2c_tick notif (st with fnums := fnums)))) (i2c fext fbits (SUC n))
+      /\ i2c_hw_write_rel (st with fnums := fnums).regs (OUTR (i2c_tick notif (st with fnums := fnums))).regs
+                          (i2c fext fbits n).hw2reg
+      /\ ~i2c_win_error (i2c fext fbits n).win_buses)
 
   (* We phrase it this way instead of as i2c_circuit_init fbits so that
    * combinational signals are set instead of being random values from fbits. *)
   /\ i2c_state_rel st (i2c fext fbits 0)
   /\ (!i. i < LENGTH reqs ==>
-    let
-      req = reg_req_decode (fext i).reg_req_i: 7 reg_req;
-    in
-      ~i2c_req_error req /\ cheshire_req_rel (EL i reqs) req)
+    cheshire_req_rel (EL i reqs) (reg_req_decode (fext i).reg_req_i: 7 reg_req))
+  /\ ISR (cheshire_run i2c_tick i2c_read i2c_write st reqs)
 
   ==> ?fnums. let
       (st', rdatas) = OUTR (cheshire_run i2c_tick i2c_read i2c_write (st with fnums := fnums) reqs)
@@ -565,49 +782,43 @@ Proof
              >> iff_tac
              >- simp []
              >- (rpt strip_tac >> Cases_on `i = n` >> simp []))
-      >> fs [listTheory.EL_SNOC, listTheory.EL_LENGTH_SNOC]
-
-      (* Show that `cheshire_run = INR _`. *)
-      >> `!st req. MEM req reqs ==> ISR (cheshire_req i2c_read i2c_write st req)`
-         by (simp [listTheory.MEM_EL]
-             >> rpt strip_tac
-             >> qpat_x_assum `!i. i < LENGTH reqs ==> _` $ drule_then strip_assume_tac
-             >> drule cheshire_req_i2c_req_error
-             >> simp [Excl "NOT_ISL_ISR", GSYM sumTheory.NOT_ISL_ISR])
-      >> drule_then (qspecl_then [`i2c_tick`, `st with fnums := fnums`] assume_tac) cheshire_run_cheshire_req_ISR
-      >> drule_then strip_assume_tac (iffLR sumExtraTheory.ISR_exists)
-      >> fs []
+      >> drule_then assume_tac (iffRL i2c_cheshire_run_ISR_fnums)
+      >> gs [listTheory.EL_SNOC, listTheory.EL_LENGTH_SNOC, cheshire_run_ISR_SNOC, INR_imp_ISR]
       >> pairarg_tac
       >> fs []
 
-      (* Infer from `~i2c_req_error` that `cheshire_req = INR _`, so that it can be
-       * used by `drule_all i2c_reg_top_i2c_state_rel_step`. *)
-      >> drule_all_then strip_assume_tac i2c_reg_top_rsp_correct
-      >> drule_then assume_tac i2c_reg_top_rsp_ready_error
-      >> gs []
-      >> drule_then (qx_choose_then `oracle_res` assume_tac) (iffLR sumExtraTheory.ISR_exists)
-      >> PairCases_on `oracle_res`
+      (* Then find `fnums'`, the fnums which need to follow `fnums` for the last step
+       * to keep things lining up. *)
+      >> qpat_x_assum `!fnums. ?st' rdatas st_upd notif rdata. _` $ qspec_then `fnums` strip_assume_tac
+      >> gvs []
       >> drule_all_then strip_assume_tac i2c_reg_top_i2c_state_rel_step
 
-      (* Now we have `fnums'`, the `fnums` needed for the last step to keep things
-       * lining up, and we want to use `qexists` with `fnums'` glued onto the end of
-       * `fnums`. But first, we need to find out where that end is. *)
-      >> `!st req. MEM req reqs ==> ISR (cheshire_req i2c_read i2c_write st req)`
-         by (simp [listTheory.MEM_EL]
-             >> rpt strip_tac
-             >> qpat_x_assum `!i. i < LENGTH reqs ==> _` $ drule_then strip_assume_tac
-             >> drule cheshire_req_i2c_req_error
-             >> simp [Excl "NOT_ISL_ISR", GSYM sumTheory.NOT_ISL_ISR])
-      >> drule_then (qspec_then `st with fnums := fnums` strip_assume_tac) cheshire_run_unused_fnums_2
+      (* Now we want to use `qexists` with `fnums'` glued onto the end of `fnums`; but
+       * first, we need to find out where that end is. *)
+      >> drule_then strip_assume_tac cheshire_run_unused_fnums
+      >> fs []
       >> qexists `\i. if i < n then fnums i else fnums' (i - n)`
 
-      >> first_assum $ qspec_then `\i. if i < n then fnums i else fnums' (i - n)` assume_tac
-      (* Instantiate it a second time to prove that st'' = st'. *)
-      >> first_x_assum $ qspec_then `fnums` assume_tac
-      >> gs [cheshire_run_SNOC, i2c_cheshire_req_fnums]
-      >> drule_then assume_tac cheshire_run_LENGTH_rdatas
-      >> first_x_assum (assume_tac o GSYM)
-      >> fs [i2c_cheshire_req_fnums, SF ETA_ss, listTheory.EL_SNOC, listTheory.EL_LENGTH_SNOC])
+      (* Obtain the values of `st'` and `rdatas`. *)
+      >> simp [cheshire_run_SNOC, sum_bind_def, i2c_cheshire_req_fnums, ETA_THM]
+      >> `?st. i2c_tick notif' (st'' with fnums := fnums') = INR st` by simp [GSYM ISR_exists, i2c_tick_ISR_fnums]
+      >> simp [sum_bind_def]
+
+      (* Now that we've actually got all the values we're working with, we can prove
+       * the goal. *)
+      (* st -> st'' -> st_upd' st'³' *)
+      >> qpat_x_assum `!fnums'. _ => cheshire_run _ _ _ _ _ = INR _` $ qspec_then `\i. if i < n then fnums i else fnums' (i - n)` assume_tac
+      >> fs []
+      >> drule_all_then strip_assume_tac i2c_reg_top_rsp_correct
+      >> rfs []
+
+      (* rdata *)
+      >> drule_then (assume_tac o GSYM) cheshire_run_LENGTH_rdatas
+      >> gs [listTheory.EL_SNOC, listTheory.EL_LENGTH_SNOC]
+
+      (* error *)
+      >> rpt strip_tac
+      >> fs [GSYM sumTheory.NOT_ISR_ISL, Excl "NOT_ISR_ISL"])
 QED
 
 val _ = export_theory ();
