spi_host/spi_hostCircuitScript.sml
@@ -24,8 +24,10 @@ val init_tm = add_x_inits ``
     regs := ^spi_host_regs_init_tm;
     reg2hw := ^spi_host_reg2hw_init_tm;
     (* TODO: these should be 'x too, but add_x_inits doesn't like reg_req *)
-    reg_req_win_rxdata := <| addr := 0w; |>;
-    reg_req_win_txdata := <| addr := 0w; |>;
+    win_buses := <|
+      reg_req_win_rxdata := <| addr := 0w; |>;
+      reg_req_win_txdata := <| addr := 0w; |>;
+    |>
   |>
 ``;
 
