spi_host/spi_hostCircuitStateScript.sml
@@ -40,10 +40,7 @@ Datatype:
      * same as the ones in real hardware). *)
     reg2hw: spi_host_reg2hw;
     hw2reg: spi_host_hw2reg;
-    reg_req_win_rxdata: 48 reg_req;
-    reg_req_win_txdata: 48 reg_req;
-    reg_rsp_win_rxdata: reg_rsp;
-    reg_rsp_win_txdata: reg_rsp;
+    win_buses: spi_host_win_buses;
 
     (* The decoded fields of `reg_req_i`. *)
     addr: word6;
